Metatheory.v
@@ -1,0 +1,228 @@
+Add LoadPath ".".
+
+Require Import SysF.
+Require Import Arith.
+Require Import Omega.
+
+Lemma cumulativity : forall e : env, forall t : typ, forall k k' : kind,
+                       kinding e t k -> k <= k' -> kinding e t k'.
+  intro e0. intro t. generalize e0 as e. clear e0. (* This is ugly *)
+  induction t.
+  + {
+      intros.
+      simpl.
+      simpl in H.
+      remember (get_kind e n) as k1 in H |- *.
+      destruct k1.
+      - split. apply H. destruct H. omega.
+      - apply H.
+    }
+  + {
+      intros.
+      simpl in H.
+      destruct H. destruct H. destruct H. destruct H1.
+      simpl.
+      specialize (IHt1 e x k' H1).
+      specialize (IHt2 e x0 k' H2).
+      exists k'. exists k'.
+      split. auto with arith. split.
+      apply IHt1. assert (x <= max x x0). auto with arith. omega.
+      apply IHt2. assert (x0 <= max x x0). auto with arith. omega.
+    }
+  + {
+      intros.
+      simpl.
+      simpl in H. destruct H. destruct H.
+      exists (k' - k0 + (max x k)). split.
+      apply (IHt (etvar k e) x). apply H.
+      assert (x <= max x k). auto with arith. omega.
+      assert (max x k >= k). auto with arith. assert (k' - k0 + max x k >= k). omega.
+      assert (max (k' - k0 + max x k) k = (k' - k0+ max x k)). auto with arith. rewrite H4.
+      rewrite -> H1. assert (S (k' - S (max x k) + max x k) = k' - S (max x k) + S (max x k)).
+      rewrite (plus_comm (k' - S (max x k)) (S (max x k))). rewrite le_plus_minus_r. omega.
+      omega.
+      rewrite -> H5. rewrite (plus_comm). rewrite le_plus_minus_r. trivial.
+      rewrite <- H1. apply H0.
+    }
+Qed.
+
+Fixpoint insert_kind (v : nat) (e : env) (e' : env) : Prop :=
+  match (e, e') with
+    | (evar t e1, evar t' e1') => (tshift v t) = t' /\ insert_kind v e1 e1'
+    | (etvar k e1, etvar k' e1') =>
+      match v with
+        | 0 => etvar k e1 = e1'
+        | S v1 => k = k' /\ insert_kind v1 e1 e1'
+      end
+    | (empty, etvar k empty) => v = 0
+    | _ => False
+  end.
+
+Lemma get_kind_Sv : forall (v : nat), forall e : env, get_kind e (S v) <> None -> get_kind e v <> None.
+  intros until e. generalize v. induction e.
+  - intros. simpl in H. simpl. apply H.
+  - intros. simpl. simpl in H. apply (IHe v0). apply H.
+  - intros. destruct v0.
+    + simpl. intro. inversion H0.
+    + simpl. simpl in H.  apply IHe. apply H.
+Qed.
+
+Lemma get_kind_etvar : forall e : env, forall v : nat, get_kind e v <> None ->
+                                                       forall k : kind, get_kind (etvar k e) v <> None.
+  intro. induction e.
+  - intros. destruct v; [ simpl in H; exfalso; apply H; reflexivity .. ].
+  - intros. destruct v.
+    + simpl. intro. inversion H0.
+    + simpl. simpl in H. apply get_kind_Sv. apply H.
+  - intros. destruct v.
+    + simpl. intro. inversion H0.
+    + simpl. destruct v.
+      * simpl. intro. inversion H0.
+      * simpl. simpl in H. apply get_kind_Sv. apply H.
+Qed.
+
+Lemma get_kind_evar : forall e : env, forall v : nat, get_kind e v <> None ->
+                                                      forall t : typ, get_kind (evar t e) v <> None.
+  intro. induction e.
+  - intros. destruct v; [ simpl in H; exfalso; apply H; reflexivity .. ].
+  - intros. simpl in H. simpl. apply H.
+  - intros. simpl. apply H.
+Qed.
+
+Definition fix_var (v : nat) (i : nat) :=
+  if le_gt_dec i v
+  then S v
+  else v.
+
+Lemma get_kind_fix_var : forall (v i : nat), forall (e : env),
+                          get_kind e v <> None -> get_kind e (S v) <> None ->
+                          get_kind e (fix_var v i) <> None.
+  intros.
+  unfold fix_var.
+  destruct (le_gt_dec i v).
+  auto.
+  auto.
+Qed.
+
+Lemma get_kind_Sn : forall (e : env), forall (v : nat), get_kind e (S v) <> None -> get_kind e v <> None.
+  induction e.
+  - intros. exfalso. apply H. trivial.
+  - intros. apply IHe. apply H.
+  - intros. destruct v; [ intro; inversion H0 | apply IHe; apply H ].
+Qed.
+
+Lemma insert_kind_get_kind_etvar : forall (e e' : env), forall (v : nat),
+                                  insert_kind v e e' ->
+                                  forall (w : nat), forall (k : kind),
+                                    get_kind (etvar k e) w <> None -> get_kind e' w <> None.
+  induction e.
+  - intros. destruct e'.
+    + inversion H.
+    + inversion H.
+    + destruct w.
+      { simpl. intro. inversion H1. }
+      { simpl. simpl H. destruct e'.
+        * simpl. auto.
+        * simpl in H. auto.
+        * inversion H. }
+  - intros. destruct e'.
+    + inversion H.
+    + simpl in H. simpl. apply (fun h => IHe e' v h w k). apply H.
+      destruct w.
+      * simpl. auto.
+      * apply H0.
+    + inversion H.
+  - intros. destruct e'.
+    + inversion H.
+    + inversion H.
+    + destruct w.
+      * simpl. intro. inversion H1.
+      * destruct v.
+        { simpl in H. rewrite <- H. apply H0. }
+        { simpl. simpl in H. apply (fun h => IHe e' v h w k). apply H. apply H0. }
+Qed.
+
+Lemma insert_kind_get_kind_Sn : forall (e e' : env), forall (v : nat),
+                                  insert_kind v e e' -> forall (w : nat), get_kind e w <> None -> get_kind e' (S w) <> None.
+  intros.
+  apply (insert_kind_get_kind_etvar e e' v H (S w) 0).
+  apply H0.
+Qed.
+
+Lemma insert_kind_get_kind_n : forall (e e' : env), forall (v : nat),
+                                 insert_kind v e e' -> forall (w : nat), get_kind e w <> None -> get_kind e' w <> None.
+  intros.
+  apply (insert_kind_get_kind_etvar e e' v H w 0).
+  apply get_kind_etvar.
+  auto.
+Qed.
+
+Lemma insert_kind_get_kind : forall (e e' : env), forall (v : nat),
+                                 insert_kind v e e' ->
+                                 forall (w : nat), get_kind e w <> None -> get_kind e' (fix_var w v) <> None.
+  intros.
+  apply get_kind_fix_var.
+  apply (insert_kind_get_kind_n e e' v). auto. auto.
+  apply (insert_kind_get_kind_Sn e e' v). auto. auto.
+Qed.
+
+Lemma insert_kind_wf_typ : forall (t : typ), forall (e e' : env), forall (v : nat), insert_kind v e e' ->
+                                                                  wf_typ e t -> wf_typ e' (tshift v t).
+  induction t.
+  - intros.
+    simpl.
+    pose proof (insert_kind_get_kind e e' v H n).
+    simpl in H0.
+    destruct (get_kind e n).
+    + unfold fix_var in H1.
+      remember (get_kind e' (if le_gt_dec v n then S n else n)) in H1 |- *.
+      destruct o.
+      * trivial.
+      * apply H1. intro. inversion H2. auto.
+    + inversion H0.
+  - intros.
+    simpl.
+    simpl in H0.
+    split.
+    { apply (IHt1 e e' v). apply H. apply H0. }
+    { apply (IHt2 e e' v). apply H. apply H0. }
+  - intros.
+    simpl.
+    simpl in H0.
+    apply (IHt (etvar k e) (etvar k e') (S v)).
+    simpl.
+    split.
+    trivial.
+    apply H.
+    apply H0.
+Qed. 
+
+Theorem insert_kind_wf_env : forall (v : nat), forall (e e' : env), insert_kind v e e' -> wf_env e -> wf_env e'.
+  intros until e. generalize v. clear v.
+  induction e.
+  - intros. destruct e'.
+    + inversion H.
+    + inversion H.
+    + simpl in H. destruct e'.
+      * trivial.
+      * inversion H.
+      * inversion H.
+  - intros. destruct e'.
+    + simpl. trivial.
+    + simpl. split. 
+      * simpl in H.
+        simpl in H0.
+        destruct H.
+        rewrite <- H.
+        apply (insert_kind_wf_typ t e).
+        apply H1.
+        apply H0.
+      * apply (IHe v). apply H. apply H0.
+    + inversion H.
+  - intros. destruct e'.
+    + simpl. trivial.
+    + inversion H.
+    + destruct v.
+      * simpl in H. rewrite <- H. simpl. apply H0.
+      * simpl in H. simpl. apply (IHe v e'). apply H. apply H0.
+Qed.
